Update heap resources for fixing Load's FTLR

theories/model/heap_ghost.v
@@ -1,4 +1,4 @@
-From griotte Require Export heap_std.
+From griotte Require Export heap_std compartment_names.
 From iris.algebra Require Import auth agree gmap gset.
 From iris.base_logic Require Export invariants.
 From iris.proofmode Require Import proofmode.
@@ -15,7 +15,10 @@ Definition heap_encode (W_heap : Heap) : heapUR :=
   (to_agree <$> heap_bounds W_heap, heap_quarantined W_heap).
 
 Class heap_preG Σ := { heap_inG :: inG Σ heap_authUR }.
-Class heapG Σ := { heap_pre_inG :: heap_preG Σ; heap_name : gname }.
+Class heapG Σ `{CmptNameG} := {
+  heap_pre_inG :: heap_preG Σ;
+  heap_name : CmptName -> gname;
+}.
 Definition heapΣ := #[GFunctor heap_authUR].
 Global Instance subG_heapΣ Σ : subG heapΣ Σ -> heap_preG Σ.
 Proof. solve_inG. Qed.
@@ -82,49 +85,49 @@ Proof.
 Qed.
 
 Section heap_ghost.
-  Context {Σ : gFunctors} {heapg : heapG Σ}.
+  Context {Σ : gFunctors} {Cname : CmptNameG} {heapg : heapG Σ}.
 
-  (** Authority is held once for the global heap. Snapshots are lower bounds:
+  (** Each compartment owns its heap authority. Snapshots are lower bounds:
       a live snapshot records bounds but makes no assertion of current liveness. *)
-  Definition heap_std_auth (W_heap : Heap) : iProp Σ :=
-    ⌜heap_wf W_heap⌝ ∗ own heap_name (● heap_encode W_heap).
-  Definition heap_std_full (W_heap : Heap) : iProp Σ :=
-    ⌜heap_wf W_heap⌝ ∗ own heap_name (◯ heap_encode W_heap).
+  Definition heap_std_auth (C : CmptName) (W_heap : Heap) : iProp Σ :=
+    ⌜heap_wf W_heap⌝ ∗ own (heap_name C) (● heap_encode W_heap).
+  Definition heap_std_full (C : CmptName) (W_heap : Heap) : iProp Σ :=
+    ⌜heap_wf W_heap⌝ ∗ own (heap_name C) (◯ heap_encode W_heap).
 
-  Global Instance heap_std_auth_timeless W_heap : Timeless (heap_std_auth W_heap).
+  Global Instance heap_std_auth_timeless C W_heap : Timeless (heap_std_auth C W_heap).
   Proof. apply _. Qed.
-  Global Instance heap_std_full_timeless W_heap : Timeless (heap_std_full W_heap).
+  Global Instance heap_std_full_timeless C W_heap : Timeless (heap_std_full C W_heap).
   Proof. apply _. Qed.
-  Global Instance heap_std_full_persistent W_heap : Persistent (heap_std_full W_heap).
+  Global Instance heap_std_full_persistent C W_heap : Persistent (heap_std_full C W_heap).
   Proof. apply _. Qed.
 
-  Lemma heap_std_auth_full W_heap :
-    heap_std_auth W_heap ==∗ heap_std_auth W_heap ∗ heap_std_full W_heap.
+  Lemma heap_std_auth_full C W_heap :
+    heap_std_auth C W_heap ==∗ heap_std_auth C W_heap ∗ heap_std_full C W_heap.
   Proof.
     iIntros "[%Hwf Ha]". iMod (own_update _ _ (● heap_encode W_heap ⋅ ◯ heap_encode W_heap) with "Ha") as "[Ha Hs]".
     { apply auth_update_dfrac_alloc; [apply _|reflexivity]. }
     iModIntro. iFrame. auto.
   Qed.
 
-  Lemma heap_std_full_weaken W_heap W_heap' :
+  Lemma heap_std_full_weaken C W_heap W_heap' :
     heap_wf W_heap -> related_sts_heap_std W_heap W_heap' ->
-    heap_std_full W_heap' -∗ heap_std_full W_heap.
+    heap_std_full C W_heap' -∗ heap_std_full C W_heap.
   Proof.
     iIntros (Hwf Hrel) "[_ Hs]". iSplit; first done.
     iApply (own_mono with "Hs"). apply auth_frag_mono, heap_encode_mono; done.
   Qed.
 
-  Lemma heap_std_auth_full_related W_heap W_heap_old :
-    heap_std_auth W_heap -∗ heap_std_full W_heap_old -∗ ⌜related_sts_heap_std W_heap_old W_heap⌝.
+  Lemma heap_std_auth_full_related C W_heap W_heap_old :
+    heap_std_auth C W_heap -∗ heap_std_full C W_heap_old -∗ ⌜related_sts_heap_std W_heap_old W_heap⌝.
   Proof.
     iIntros "[%Hwf Ha] [_ Hs]".
     iDestruct (own_valid_2 with "Ha Hs") as %[Hincl _]%auth_both_valid_discrete.
     iPureIntro. by apply heap_encode_future.
   Qed.
 
-  Lemma heap_std_auth_update W_heap W_heap' :
+  Lemma heap_std_auth_update C W_heap W_heap' :
     related_sts_heap_std W_heap W_heap' ->
-    heap_std_auth W_heap ==∗ heap_std_auth W_heap' ∗ heap_std_full W_heap'.
+    heap_std_auth C W_heap ==∗ heap_std_auth C W_heap' ∗ heap_std_full C W_heap'.
   Proof.
     iIntros (Hrel) "[%Hwf Ha]".
     have Hincl := heap_encode_mono W_heap W_heap' Hrel.
@@ -139,24 +142,40 @@ Section heap_ghost.
     iModIntro. iFrame. auto.
   Qed.
 
-  Lemma heap_std_auth_allocate W_heap b e :
+  Lemma heap_std_auth_allocate C W_heap b e :
     heap_fresh W_heap b e ->
-    heap_std_auth W_heap ==∗ heap_std_auth (heap_allocate W_heap b e) ∗
-      heap_std_full (heap_allocate W_heap b e).
+    heap_std_auth C W_heap ==∗ heap_std_auth C (heap_allocate W_heap b e) ∗
+      heap_std_full C (heap_allocate W_heap b e).
   Proof. intros Hfresh. apply heap_std_auth_update, heap_allocate_future; done. Qed.
 
-  Lemma heap_std_auth_quarantine W_heap b :
-    heap_std_auth W_heap ==∗ heap_std_auth (heap_quarantine W_heap b) ∗
-      heap_std_full (heap_quarantine W_heap b).
+  Lemma heap_std_auth_quarantine C W_heap b :
+    heap_std_auth C W_heap ==∗ heap_std_auth C (heap_quarantine W_heap b) ∗
+      heap_std_full C (heap_quarantine W_heap b).
   Proof. apply heap_std_auth_update, heap_quarantine_future. Qed.
 End heap_ghost.
 
-Lemma heap_std_init {Σ : gFunctors} {heappreg : heap_preG Σ} :
-  ⊢ |==> ∃ heapg : heapG Σ, heap_std_auth ∅ ∗ heap_std_full ∅.
+Lemma heap_std_init {Σ : gFunctors} {Cname : CmptNameG} {heappreg : heap_preG Σ} :
+  ⊢ |==> ∃ heapg : heapG Σ,
+    [∗ set] C ∈ CNames, heap_std_auth C ∅ ∗ heap_std_full C ∅.
 Proof.
-  iMod (own_alloc (● heap_encode ∅ ⋅ ◯ heap_encode ∅)) as (γ) "[Ha Hs]".
-  { apply auth_both_valid_discrete. split; first done. apply heap_encode_valid. }
-  iExists (Build_heapG Σ heappreg γ). iModIntro.
+  assert (⊢ |==> ∃ γ : CmptName -> gname,
+    [∗ set] C ∈ CNames, own (γ C) (● heap_encode ∅ ⋅ ◯ heap_encode ∅))%I as Hinit.
+  { induction CNames as [|C Cs HC IH] using set_ind_L.
+    - iModIntro. iExists (λ C, encode C). by iApply big_sepS_empty.
+    - iMod IH as (γ) "Hnames".
+      iMod (own_alloc (● heap_encode ∅ ⋅ ◯ heap_encode ∅)) as (γC) "Hnew".
+      { apply auth_both_valid_discrete. split; first done. apply heap_encode_valid. }
+      iModIntro.
+      iExists (λ C', if bool_decide (C' = C) then γC else γ C').
+      iApply (big_sepS_union_2 with "[Hnew]").
+      + iApply big_sepS_singleton. by rewrite bool_decide_eq_true_2.
+      + iApply (big_sepS_mono with "Hnames").
+        iIntros (C' HC') "Hname".
+        rewrite bool_decide_eq_false_2; [done|set_solver]. }
+  iMod Hinit as (γ) "Hnames".
+  iExists (Build_heapG Σ Cname heappreg γ). iModIntro.
+  iApply (big_sepS_mono with "Hnames").
+  iIntros (C HC) "[Ha Hs]".
   rewrite /heap_std_auth /heap_std_full /=. iFrame.
   iSplit; iPureIntro; apply heap_wf_empty.
 Qed.
