theories/model/compartment_names.v
@@ -1,0 +1,9 @@
+From stdpp Require Import finite gmap.
+
+Class CmptNameG := CmptNameS {
+  CmptName : Type;
+  CmptName_eq_dec :: EqDecision CmptName;
+  CmptName_countable :: Finite CmptName;
+}.
+
+Definition CNames `{CmptNameG} : gset CmptName := list_to_set (enum CmptName).
